guarded.v
@@ -1,0 +1,128 @@
+From mathcomp Require Import ssreflect.
+From iris.base_logic.lib Require Import auth.
+From iris.base_logic Require Import proofmode.
+From iris.proofmode Require Import tactics.
+From iris_string_ident Require Import ltac2_string_ident.
+
+Section Guarded.
+
+Context `{Σ : gFunctors}.
+Notation iProp := (iProp Σ).
+
+Implicit Types (P Q : iProp) (G : Prop).
+
+Definition guarded G `{Decision G} P : iProp :=
+  (if decide G then P else emp)%I.
+
+Lemma guarded_leq G1 G2 `{Decision G1, Decision G2} P :
+  (G2 → G1) →
+  guarded G1 P -∗ guarded G2 P.
+Proof.
+rewrite /guarded.
+case: (decide G1) (decide G2) => [yes1|no1] [yes2|no2] //= H12;
+iIntros "H //"; by case: (no1 (H12 yes2)).
+Qed.
+
+Context `{!Decision G}.
+
+Global Instance guarded_persistent P :
+  Persistent P →
+  Persistent (guarded G P).
+Proof. rewrite /guarded; case: decide => //= _; apply _. Qed.
+
+Lemma guarded_sep P Q :
+  guarded G (P ∗ Q) ⊣⊢ guarded G P ∗ guarded G Q.
+Proof.
+rewrite /guarded; case: decide => /=; eauto.
+by rewrite -bi.intuitionistically_emp -bi.intuitionistically_sep_dup.
+Qed.
+
+Global Instance guarded_from_sep P Q R :
+  FromSep P Q R →
+  FromSep (guarded G P) (guarded G Q) (guarded G R).
+Proof.
+rewrite {2}/FromSep; iIntros (FS) "H".
+rewrite -guarded_sep /guarded; case: decide => //= _.
+by iApply from_sep.
+Qed.
+
+Global Instance guarded_into_sep P Q R :
+  IntoSep P Q R →
+  IntoSep (guarded G P) (guarded G Q) (guarded G R).
+Proof.
+rewrite {2}/IntoSep; iIntros (FS) "H".
+rewrite -guarded_sep /guarded; case: decide => //= _.
+by iApply into_sep.
+Qed.
+
+Global Instance guarded_into_and b (P Q R : iProp) :
+  IntoAnd b P Q R →
+  IntoAnd b (guarded G P) (guarded G Q) (guarded G R).
+Proof.
+rewrite /guarded.
+by case: b (decide G) => [] //= [] _ //= _; rewrite /IntoAnd /=; eauto.
+Qed.
+
+Lemma guarded_fupd `{!invG Σ} E P :
+  guarded G (|={E}=> P) ⊣⊢ |={E}=> guarded G P.
+Proof.
+rewrite /guarded.
+by case: decide => //= _; apply (anti_symm _); iIntros => //.
+Qed.
+
+Lemma guarded_later P :
+  guarded G (▷ P) ⊣⊢ ▷ guarded G P.
+Proof.
+rewrite /guarded.
+by case: decide => //= _; rewrite bi.later_emp.
+Qed.
+
+Lemma guarded_mono P Q :
+  guarded G P -∗
+  □ (P -∗ Q) -∗
+  guarded G Q.
+Proof.
+rewrite /guarded.
+iIntros "HP #PQ"; by case: decide => // _; iApply "PQ".
+Qed.
+
+Lemma guarded_exist T (φ : T -> iProp) :
+  Inhabited T →
+  guarded G (∃ x : T, φ x) ⊣⊢ ∃ x : T, guarded G (φ x).
+Proof.
+rewrite /guarded.
+move=> ?; case: decide=> //= _.
+apply (anti_symm _); last by eauto.
+by iIntros "_"; iExists inhabitant.
+Qed.
+
+Global Instance guarded_from_exist T (φ : T -> iProp) :
+  Inhabited T →
+  FromExist (guarded G (∃ x, φ x)) (λ x, guarded G (φ x)).
+Proof.
+by move => ?; rewrite /FromExist guarded_exist.
+Qed.
+
+Global Instance guarded_into_exist T (φ : T -> iProp) :
+  Inhabited T →
+  IntoExist (guarded G (∃ x, φ x)) (λ x, guarded G (φ x)).
+Proof.
+by move => ?; rewrite /IntoExist guarded_exist.
+Qed.
+
+Lemma guarded_box (P : iProp) : □ guarded G P ⊣⊢ guarded G (□ P).
+Proof.
+rewrite /guarded.
+case: decide => //= _; by rewrite bi.intuitionistically_emp.
+Qed.
+
+Global Instance guarded_box_into_persistent p (P Q : iProp) :
+  IntoPersistent p P Q →
+  IntoPersistent p (guarded G P) (guarded G Q).
+Proof.
+rewrite /guarded.
+case: decide => //= _ _.
+by rewrite /IntoPersistent; rewrite -bi.persistently_emp_intro; eauto.
+Qed.
+
+End Guarded.
